CorrectnessUpd.thy
@@ -1,0 +1,136 @@
+theory CorrectnessUpd
+imports "Denotational-PropsUpd" "Launchbury"
+begin
+
+theorem correctness:
+  assumes "\<Gamma> : e \<Down>\<^bsub>L\<^esub> \<Delta> : z"
+  and     "distinctVars \<Gamma>"
+  and     "fdom \<rho> - heapVars \<Gamma> \<subseteq> set L"
+  shows   "\<lbrakk>e\<rbrakk>\<^bsub>\<lbrace>\<Gamma>\<rbrace>\<rho>\<^esub> = \<lbrakk>z\<rbrakk>\<^bsub>\<lbrace>\<Delta>\<rbrace>\<rho>\<^esub>" and "\<lbrace>\<Gamma>\<rbrace>\<rho> \<le> \<lbrace>\<Delta>\<rbrace>\<rho>"
+  using assms
+proof(nominal_induct avoiding: \<rho> rule:reds_distinct_strong_ind)
+case (Lambda \<Gamma> x e L \<rho>)
+  case 1 show ?case by rule
+  case 2 show ?case by rule
+next
+case (Application y \<Gamma> e x L \<Delta> \<Theta> z e' \<rho>)
+  hence [simp]:"atom y \<sharp> \<lbrace>\<Delta>\<rbrace>\<rho>" and "y \<noteq> x"
+    by (simp_all add: fresh_at_base)
+
+  case 1
+  hence hyp1: "fdom \<rho> - heapVars \<Gamma> \<subseteq> set (x # L)" by auto
+  have hyp2: "fdom \<rho> - heapVars \<Delta> \<subseteq> set L"
+    using 1 reds_doesnt_forget[OF distinct_redsD1[OF Application.hyps(9)]]
+    by auto
+
+  have [simp]: "the (lookup (\<lbrace>\<Gamma>\<rbrace>\<rho>) x) = the (lookup (\<lbrace>\<Delta>\<rbrace>\<rho>) x)"
+  proof(cases "x \<in> heapVars \<Gamma>")
+  case True
+    thus ?thesis
+      by (simp add: fmap_less_eqD[OF Application.hyps(11)[OF hyp1]] heapVars_def)
+  next
+  case False
+    have "x \<notin> heapVars \<Delta>"
+      by (rule reds_avoids_live[OF distinct_redsD1[OF Application.hyps(9)] _ False], simp)
+    with False
+    show ?thesis
+      by (simp add: the_lookup_HSem_other heapVars_def)
+  qed
+
+  have "\<lbrakk> App e x \<rbrakk>\<^bsub>\<lbrace>\<Gamma>\<rbrace>\<rho>\<^esub> = \<lbrakk> e \<rbrakk>\<^bsub>\<lbrace>\<Gamma>\<rbrace>\<rho>\<^esub> \<down>Fn \<lbrakk> Var x \<rbrakk>\<^bsub>\<lbrace>\<Gamma>\<rbrace>\<rho>\<^esub>"
+    by simp
+  also have "\<dots> = \<lbrakk> Lam [y]. e' \<rbrakk>\<^bsub>\<lbrace>\<Delta>\<rbrace>\<rho>\<^esub> \<down>Fn \<lbrakk> Var x \<rbrakk>\<^bsub>\<lbrace>\<Gamma>\<rbrace>\<rho>\<^esub>"
+    by (rule arg_cong[OF Application.hyps(10)[OF hyp1]])
+  also have "\<dots> = \<lbrakk> Lam [y]. e' \<rbrakk>\<^bsub>\<lbrace>\<Delta>\<rbrace>\<rho>\<^esub> \<down>Fn \<lbrakk> Var x \<rbrakk>\<^bsub>\<lbrace>\<Delta>\<rbrace>\<rho>\<^esub>"
+    by simp
+  also have "... = \<lbrakk> e' \<rbrakk>\<^bsub>(\<lbrace>\<Delta>\<rbrace>\<rho>)(y f\<mapsto> \<lbrakk> Var x \<rbrakk>\<^bsub>\<lbrace>\<Delta>\<rbrace>\<rho>\<^esub>)\<^esub>"
+    by simp
+  also have "... = \<lbrakk> e'[y ::= x] \<rbrakk>\<^bsub>\<lbrace>\<Delta>\<rbrace>\<rho>\<^esub>"
+    by (rule ESem_subst[OF `y \<noteq> x` `atom y \<sharp> \<lbrace>\<Delta>\<rbrace>\<rho>`])
+  also have "\<dots> = \<lbrakk> z \<rbrakk>\<^bsub>\<lbrace>\<Theta>\<rbrace>\<rho>\<^esub>"
+    by (rule Application.hyps(13)[OF hyp2])
+  finally
+  show ?case.
+  
+  case 2
+  show ?case using Application hyp1 hyp2
+    by (metis order_trans)
+next
+case (Variable x e \<Gamma> L \<Delta> z \<rho>)
+  case 2
+  have "\<lbrace>\<Gamma>\<rbrace>\<rho> = \<lbrace>(x,e) # delete x \<Gamma>\<rbrace>\<rho>"
+    sorry
+  also have "\<dots> = fix_on' (fmap_bottom (fdom \<rho> \<union> insert x (fst `set \<Gamma>)))
+    (\<lambda> \<rho>'. (\<rho> f++ fmap_restr (fst ` set \<Gamma>) (\<lbrace>delete x \<Gamma>\<rbrace>\<rho>'))( x f\<mapsto> \<lbrakk> e \<rbrakk>\<^bsub>\<rho>'\<^esub>))"
+    sorry
+  also have "\<dots> = fix_on' (fmap_bottom (fdom \<rho> \<union> insert x (fst `set \<Gamma>)))
+    (\<lambda> \<rho>'. (\<rho> f++ fmap_restr (fst ` set \<Gamma>) (\<lbrace>delete x \<Gamma>\<rbrace>\<rho>'))( x f\<mapsto> \<lbrakk> e \<rbrakk>\<^bsub>\<lbrace>delete x \<Gamma>\<rbrace>\<rho>'\<^esub>))"
+    sorry
+  also have "\<dots> = fix_on' (fmap_bottom (fdom \<rho> \<union> insert x (fst `set \<Gamma>)))
+    (\<lambda> \<rho>'. (\<rho> f++ fmap_restr (fst ` set \<Gamma>) (\<lbrace>delete x \<Gamma>\<rbrace>\<rho>'))( x f\<mapsto> \<lbrakk> z \<rbrakk>\<^bsub>\<lbrace>\<Delta>\<rbrace>\<rho>'\<^esub>))"
+    apply (rule fix_on_cong[OF _ arg_cong[OF  Variable.hyps(3)]])
+    sorry
+  also have "\<dots> \<le> fix_on' (fmap_bottom (fdom \<rho> \<union> insert x (fst `set \<Gamma>)))
+    (\<lambda> \<rho>'. (\<rho> f++ fmap_restr (fst ` set \<Gamma>) (\<lbrace>\<Delta>\<rbrace>\<rho>'))( x f\<mapsto> \<lbrakk> z \<rbrakk>\<^bsub>\<lbrace>\<Delta>\<rbrace>\<rho>'\<^esub>))"
+    thm Variable.hyps(4)
+    sorry
+  also have "\<dots> = fix_on' (fmap_bottom (fdom \<rho> \<union> insert x (fst `set \<Gamma>)))
+    (\<lambda> \<rho>'. (\<rho> f++ fmap_restr (fst ` set \<Gamma>) (\<lbrace>\<Delta>\<rbrace>\<rho>'))( x f\<mapsto> \<lbrakk> z \<rbrakk>\<^bsub>\<rho>'\<^esub>))"
+    sorry
+  also have "\<dots> = \<lbrace>(x,z) # \<Delta>\<rbrace>\<rho>"
+    sorry
+  finally
+  show le: ?case.
+
+  case 1
+  have "\<lbrakk> Var x \<rbrakk>\<^bsub>\<lbrace>\<Gamma>\<rbrace>\<rho>\<^esub> = \<lbrakk> Var x \<rbrakk>\<^bsub>\<lbrace>(x, z) # \<Delta>\<rbrace>\<rho>\<^esub>"
+    using le
+    sorry
+  also have "\<dots> =  \<lbrakk> z \<rbrakk>\<^bsub>\<lbrace>(x, z) # \<Delta>\<rbrace>\<rho>\<^esub>"
+    sorry
+  finally
+  show ?case.
+next
+case (Let as \<Gamma> body L \<Delta> z \<rho>)
+  case 1
+  { fix a
+    assume a: "a \<in> heapVars (asToHeap as)"
+    have "atom a \<sharp> L" 
+      by (rule Let(3)[unfolded fresh_star_def set_bn_to_atom_heapVars, rule_format, OF imageI[OF a]])
+    hence "a \<notin> set L"
+      by (metis fresh_list_elem not_self_fresh)
+    moreover
+    have "atom a \<sharp> \<Gamma>" 
+      by (rule Let(1)[unfolded fresh_star_def set_bn_to_atom_heapVars, rule_format, OF imageI[OF a]])
+    hence "a \<notin> heapVars \<Gamma>"
+      by (metis heapVars_not_fresh)
+    ultimately
+    have "a \<notin> fdom \<rho>" and "a \<notin> heapVars \<Gamma>"
+      using 1 by auto
+  }
+  hence  [simp]: "set (bn as) \<sharp>* (\<lbrace>\<Gamma>\<rbrace>\<rho>)"
+    apply (subst fresh_star_def)
+    apply (subst  set_bn_to_atom_heapVars)
+    apply (auto simp add: sharp_Env heapVars_def)
+    done
+  
+  have hyp: "fdom \<rho> - heapVars (asToHeap as @ \<Gamma>) \<subseteq> set L"
+    using 1 by auto
+
+  have "\<lbrakk> Terms.Let as body \<rbrakk>\<^bsub>\<lbrace>\<Gamma>\<rbrace>\<rho>\<^esub> = \<lbrakk> body \<rbrakk>\<^bsub>\<lbrace>asToHeap as\<rbrace>\<lbrace>\<Gamma>\<rbrace>\<rho>\<^esub>"
+    by simp
+  also have "\<dots> =  \<lbrakk> body \<rbrakk>\<^bsub>\<lbrace>asToHeap as @ \<Gamma>\<rbrace>\<rho>\<^esub>"
+    sorry
+  also have "\<dots> =  \<lbrakk> z \<rbrakk>\<^bsub>\<lbrace>\<Delta>\<rbrace>\<rho>\<^esub>"
+    by (rule Let.hyps(6)[OF hyp])
+  finally
+  show ?case.
+
+  case 2
+  have "\<lbrace>\<Gamma>\<rbrace>\<rho> \<le> \<lbrace>asToHeap as @ \<Gamma>\<rbrace>\<rho>"
+    sorry
+  also have "\<dots> \<le> \<lbrace>\<Delta>\<rbrace>\<rho>"
+    by (rule Let.hyps(7)[OF hyp])
+  finally
+  show ?case.
+qed
