Denotational-PropsUpd.thy
@@ -81,7 +81,6 @@ abbreviation HSem_syn ("\<lbrace>_\<rbrace>_"  [60,60] 60) where "\<lbrace>\<Gam
 
 abbreviation HSem_fempty  ("\<lbrace>_\<rbrace>"  [60] 60) where "\<lbrace>\<Gamma>\<rbrace> \<equiv> \<lbrace>\<Gamma>\<rbrace>fempty"
 
-
 (*
 
 lemma fresh_fmap_upd'[simp]: "\<lbrakk> atom a \<sharp> \<rho>; atom x \<sharp> a ; atom a \<sharp> v \<rbrakk> \<Longrightarrow> atom a \<sharp> \<rho>(x f\<mapsto> v)"
